UTP/ITree_THoare.thy
@@ -1,0 +1,77 @@
+section \<open> Total Correctness Hoare Logic \<close>
+
+theory ITree_THoare
+  imports ITree_Hoare
+begin
+
+definition prog_term_under :: "('e, 's) htree \<Rightarrow> ('s \<Rightarrow> bool) \<Rightarrow> bool"
+  where "prog_term_under C P = (\<forall> s. P s \<longrightarrow> terminates (C s))"
+
+definition thoare_triple :: "('s \<Rightarrow> bool) \<Rightarrow> ('e, 's) htree \<Rightarrow> ('s \<Rightarrow> bool) \<Rightarrow> bool" where
+"thoare_triple P S Q = (hoare_triple P S Q \<and> prog_term_under S P)"
+
+syntax
+  "_thoare"          :: "logic \<Rightarrow> logic \<Rightarrow> logic \<Rightarrow> logic" ("H[_]/ _/ [_]")
+
+translations
+  "_thoare P S Q" == "CONST thoare_triple (P)\<^sub>e S (Q)\<^sub>e"
+
+lemma thoare_then_hoare: "H[P] C [Q] \<Longrightarrow> H{P} C {Q}"
+  by (simp add: thoare_triple_def)
+
+lemma thoareI: "\<lbrakk> H{P} C {Q}; prog_term_under C (P)\<^sub>e \<rbrakk> \<Longrightarrow> H[P] C [Q]"
+  by (simp add: thoare_triple_def)
+
+lemma thl_conseq:
+  assumes "H[P\<^sub>2] S [Q\<^sub>2]" "`P\<^sub>1 \<longrightarrow> P\<^sub>2`" "`Q\<^sub>2 \<longrightarrow> Q\<^sub>1`"
+  shows "H[P\<^sub>1] S [Q\<^sub>1]"
+  using assms 
+  by (simp add: thoare_triple_def hoare_alt_def prog_term_under_def)
+     (expr_auto, blast)
+
+lemma thl_skip: "H[P] Skip [P]"
+  by (auto simp add: thoare_triple_def prog_term_under_def hoare_alt_def Skip_def terminates_Ret)
+
+lemma thl_skip': 
+  assumes "`P \<longrightarrow> Q`"
+  shows "H[P] Skip [Q]"
+  by (meson assms hl_skip' thl_skip thoare_triple_def)
+
+lemma thl_seq: "\<lbrakk> H[P] S\<^sub>1 [Q]; H[Q] S\<^sub>2 [R] \<rbrakk> \<Longrightarrow> H[P] S\<^sub>1 ;; S\<^sub>2 [R]"
+  by (auto simp add: thoare_triple_def hl_seq prog_term_under_def)
+     (auto intro!: terminates_bind simp add: seq_itree_def kleisli_comp_def hoare_alt_def retvals_def)
+
+lemma thl_assigns: "H[\<sigma> \<dagger> P] \<langle>\<sigma>\<rangle>\<^sub>a [P]"
+  by (metis assigns_def hoare_assigns prog_term_under_def terminates_Ret thoare_triple_def)
+
+lemma thl_assign: "H[P\<lbrakk>e/x\<rbrakk>] x := e [P]"
+  by (rule thl_assigns)
+
+lemma thl_cond [hoare_safe]:
+  assumes "H[B \<and> P] S [Q]" "H[\<not>B \<and> P] T [Q]"
+  shows "H[P] if B then S else T fi [Q]"
+  using assms
+  by (auto simp add: thoare_triple_def hl_cond)
+     (simp add: cond_itree_def prog_term_under_def)
+
+lemma thl_while [hoare_safe]:
+  fixes V :: "'s \<Rightarrow> 'a::wellorder"
+  assumes "\<And> z. H[P \<and> B \<and> V = \<guillemotleft>z\<guillemotright>] S [P \<and> V < \<guillemotleft>z\<guillemotright>]"
+  shows "H[P] while B do S od [\<not> B \<and> P]"
+proof -
+  from assms have "\<^bold>{P \<and> B\<^bold>} S \<^bold>{P\<^bold>}"
+    by (auto simp add: hoare_alt_def thoare_triple_def)
+  hence partial: "\<^bold>{P\<^bold>} while B do S od \<^bold>{\<not> B \<and> P\<^bold>}"
+    by (rule hoare_while_partial)
+  from assms have S_term: "\<And> s. \<lbrakk> B s; P s \<rbrakk> \<Longrightarrow> terminates (S s)"
+    by (simp add: thoare_triple_def SEXP_def prog_term_under_def)  
+
+  from assms have wS_term: "prog_term_under (while B do S od) P"
+    unfolding thoare_triple_def hoare_alt_def prog_term_under_def
+    by (auto intro!: terminates_iterate_wellorder_variant[of B P S V] simp add: SEXP_def)
+
+  show ?thesis
+    by (metis SEXP_def partial thoareI wS_term)
+qed
+
+end
